monadic rewrite of cheerios

Combinators.v
@@ -1,207 +1,214 @@
-Require Import StructTact.StructTactics.
 Require Import List.
+Import ListNotations.
+Require Vector String.
+
 Require Import Cheerios.Core.
+Require Import Cheerios.BasicSerializers.
+Require Import Cheerios.DeserializerMonad.
+Import DeserializerNotations.
+Require Import Cheerios.Tactics.
+
+(* These functions are either missing obvious implicits, or have
+   implicit arguments that are not marked "maximally inserted", which
+   means they cannot easily be used with map or fmap. *)
+Arguments Some {_} _.
+Arguments cons {_} _ _.
+Arguments option_map {_ _} _ _.
+Arguments Vector.nil {_}.
+Arguments Vector.cons {_} _ {_} _.
 
 Section combinators.
-  Variable A : Type.
+
+  (* This section gives instances for various type constructors, including pairs
+    and lists. *)
+  Variables A B : Type.
   Variable sA : Serializer A.
-
-  Hint Rewrite app_assoc_reverse : serialize.
-  (* Need @ on Serialize_reversible so that it doesn't bind early *)
-  Hint Rewrite @Serialize_reversible : serialize.
-
-  Ltac simplify :=
-    repeat (autorewrite with serialize; try (rewrite deserialize_preserves_input); cbn; auto).
-
-  Definition option_serialize (o: option A) :=
-    match o with
-    | None => serialize false
-    | Some t => serialize true ++ serialize t
-    end.
-
-  Definition option_deserialize (bin: list bool) : option (option A * list bool) :=
-    match deserialize bin with
-    | None => None
-    | Some (b, rest) =>
-    match b with
-    | false => Some (None, rest)
-    | true =>
-    match deserialize rest with
-    | None => None
-    | Some (t, rest) =>
-      Some (Some t, rest)
-    end
-    end
-    end.
-
-  Lemma option_deserialize_preserves_input :
-    forall (o: option A) (bin: list bool),
-      option_deserialize (option_serialize o ++ bin) = Some (o, bin).
-  Proof.
-    unfold option_deserialize, option_serialize.
-    intros o bin.
-    destruct o; simpl; auto.
-    simplify.
-  Qed.
-
-  (* Global here means "redeclare this instance outside the section."
-     If you leave this off, then the instance must be manually re-declared. *)
-  Global Instance Option_Serializer : Serializer (option A) :=
-    {
-      serialize := option_serialize;
-      deserialize := option_deserialize;
-      deserialize_preserves_input := option_deserialize_preserves_input
-    }.
-
-  Variable B : Type.
   Variable sB : Serializer B.
 
-  Definition pair_serialize (p: A*B) :=
-    let (a, b) := p in
-    (serialize a) ++ (serialize b).
-
-  Definition pair_deserialize (bin: list bool) : option ((A * B) * list bool) :=
-    match deserialize bin with
-    | None => None
-    | Some (a, rest) =>
-    match deserialize rest with
-    | None => None
-    | Some (b, remainder) =>
-      Some ((a, b), remainder)
-    end
+  Definition option_serialize (x : option A) : list bool :=
+    match x with
+    | Some a => serialize true ++ serialize a
+    | None => serialize false
     end.
 
-  Lemma pair_deserialize_preserves_input :
-    forall (p: A * B) (bin: list bool),
-      pair_deserialize (pair_serialize p ++ bin) = Some (p, bin).
+  Definition option_deserialize : deserializer (option A) :=
+    b <- deserialize ;;
+    match b with
+    | true => Some <$> deserialize
+    | false => ret None
+    end.
+
+  Lemma option_serialize_deserialize_id :
+    serialize_deserialize_id_spec option_serialize option_deserialize.
   Proof.
-    intros.
-    unfold pair_serialize.
-    break_match.
-    unfold pair_deserialize.
-    simplify.
+    unfold option_serialize, option_deserialize.
+    destruct a; serialize_deserialize_id_crush.
   Qed.
 
-  Global Instance Pair_Serializer : Serializer (A * B) :=
-    {
-      serialize := pair_serialize;
-      deserialize := pair_deserialize;
-      deserialize_preserves_input := pair_deserialize_preserves_input
-    }.
+  Global Instance option_Serializer : Serializer (option A) :=
+    {| serialize := option_serialize;
+        deserialize := option_deserialize;
+        serialize_deserialize_id := option_serialize_deserialize_id
+    |}.
 
-  Variable C : Type.
-  Variable sC : Serializer C.
+  Definition pair_serialize (x : A * B) : list bool :=
+    let (a, b) := x in serialize a ++ serialize b.
 
-  Definition triple_serialize (t: A*B*C) :=
-    let (p, c) := t in
-    let (a, b) := p in
-    (serialize a) ++ (serialize b) ++ (serialize c).
+  Definition pair_deserialize : deserializer (A * B) :=
+    liftD2 pair.
 
-  Definition triple_deserialize (bin: list bool): option ((A*B*C) * list bool) :=
-    match deserialize bin with
-    | None => None
-    | Some (a, rest) =>
-    match deserialize rest with
-    | None => None
-    | Some (b, rest) =>
-    match deserialize rest with
-    | None => None
-    | Some (c, remainder) =>
-      Some ((a, b, c), remainder)
-    end
-    end
-    end.
-
-  Lemma triple_deserialize_preserves_input :
-    forall (t: A * B * C) (bin: list bool),
-      triple_deserialize (triple_serialize t ++ bin) = Some (t, bin).
+  Lemma pair_serialize_deserialize_id :
+    serialize_deserialize_id_spec pair_serialize pair_deserialize.
   Proof.
-    intros.
-    unfold triple_serialize.
-    repeat break_match.
-    unfold triple_deserialize.
-    simplify.
+    unfold pair_serialize, pair_deserialize.
+    destruct a; serialize_deserialize_id_crush.
   Qed.
 
-  Global Instance Triple_Serializer : Serializer (A * B * C) :=
-    {
-      serialize := triple_serialize;
-      deserialize := triple_deserialize;
-      deserialize_preserves_input := triple_deserialize_preserves_input 
-    }.
+  Global Instance pair_Serializer : Serializer (A * B) :=
+    {| serialize := pair_serialize;
+        deserialize := pair_deserialize;
+        serialize_deserialize_id := pair_serialize_deserialize_id
+    |}.
 
-  Fixpoint list_serialize_rec (ts: list A) :=
-    match ts with
-    | nil => nil
-    | hd :: ts => (serialize hd) ++ (list_serialize_rec ts)
+
+  Definition sum_serialize (x : A + B) : list bool :=
+    match x with
+    | inl a => serialize true ++ serialize a
+    | inr b => serialize false ++ serialize b
     end.
 
-  Definition list_serialize (ts: list A) :=
-    serialize (length ts) ++ (list_serialize_rec ts).
-
-  Fixpoint list_deserialize_rec (count: nat) (bin: list bool) : option (list A * list bool) :=
-    match count with
-      | 0 => Some (nil, bin)
-      | S n =>
-    match deserialize bin with
-      | None => None
-      | Some (t, rest) =>
-    match list_deserialize_rec n rest with
-      | None => None
-      | Some (elements, rest) => Some ((t :: elements), rest)
-    end
-    end
+  Definition sum_deserialize : deserializer (A + B) :=
+    b <- deserialize ;;
+    match b with
+    | true => inl <$> deserialize
+    | false => inr <$> deserialize
     end.
 
-  Definition list_deserialize (bin: list bool) : option (list A * list bool) :=
-    match deserialize bin with
-    | None => None
-    | Some (count, rest) =>
-      list_deserialize_rec count rest
-    end.
-
-  Lemma list_deserialize_preserves_input :
-    forall (ts: list A) (bin: list bool),
-      list_deserialize (list_serialize ts ++ bin) = Some (ts, bin).
+  Lemma sum_serialize_deserialize_id :
+    serialize_deserialize_id_spec sum_serialize sum_deserialize.
   Proof.
-    unfold list_deserialize, list_serialize.
-    intros ts bin.
-    simplify.
-    induction ts; simplify.
-    now rewrite IHts.
+    unfold sum_serialize, sum_deserialize.
+    destruct a; serialize_deserialize_id_crush.
   Qed.
 
-  Global Instance List_Serializer : Serializer (list A) :=
-    {
-      serialize := list_serialize;
-      deserialize := list_deserialize;
-      deserialize_preserves_input := list_deserialize_preserves_input
-    }.
+  Global Instance sum_Serializer : Serializer (A + B) :=
+    {| serialize := sum_serialize;
+        deserialize := sum_deserialize;
+        serialize_deserialize_id := sum_serialize_deserialize_id
+    |}.
 
-  Variable to : B -> A.
-  Variable from : A -> B.
-  Hypothesis to_from_inverse : forall b, from (to b) = b.
 
-  Definition to_from_serialize (b : B) : list bool := serialize (to b).
-
-  Definition to_from_deserialize bin : option (B * list bool) :=
-    match deserialize(A:=A) bin with None => None
-    | Some (a, bin) => Some (from a, bin)
+  Fixpoint list_serialize_rec (l : list A) : list bool :=
+    match l with
+    | [] => []
+    | a :: l' => serialize a ++ list_serialize_rec l'
     end.
 
-  Lemma to_from_deserialize_preserves_input : forall b bin,
-      to_from_deserialize (to_from_serialize b ++ bin) = Some (b, bin).
+  Definition list_serialize (l : list A) : list bool :=
+    serialize (length l) ++ list_serialize_rec l.
+
+  Fixpoint list_deserialize_rec (n : nat) : deserializer (list A) :=
+    match n with
+    | 0 => ret []
+    | S n' => cons <$> deserialize <*> list_deserialize_rec n'
+    end.
+
+  Definition list_deserialize : deserializer (list A) :=
+    deserialize >>= list_deserialize_rec.
+
+  Lemma list_serialize_deserialize_id_rec :
+    forall l bin, list_deserialize_rec (length l) (list_serialize_rec l ++ bin) = Some (l, bin).
   Proof.
-    unfold to_from_serialize, to_from_deserialize.
-    intros b bin.
-    simplify.
-    now rewrite to_from_inverse.
+    induction l; simpl; serialize_deserialize_id_crush.
+    now rewrite IHl.
   Qed.
 
-  Global Instance To_From_Serializer : Serializer B :=
-    {
-      serialize := to_from_serialize;
-      deserialize := to_from_deserialize;
-      deserialize_preserves_input := to_from_deserialize_preserves_input
-    }.
+  Lemma list_serialize_deserialize_id :
+    serialize_deserialize_id_spec list_serialize list_deserialize.
+  Proof.
+    unfold list_serialize, list_deserialize.
+    serialize_deserialize_id_crush.
+    apply list_serialize_deserialize_id_rec.
+  Qed.
+
+  Global Instance list_Serializer : Serializer (list A) :=
+    {| serialize := list_serialize;
+        deserialize := list_deserialize;
+        serialize_deserialize_id := list_serialize_deserialize_id
+    |}.
+
+  Fixpoint vector_serialize {n} (v : Vector.t A n) : list bool :=
+    match v with
+    | Vector.nil => []
+    | Vector.cons a v' => serialize a ++ vector_serialize v'
+    end.
+
+  Fixpoint vector_deserialize {n} : deserializer (Vector.t A n) :=
+    match n as n0 return deserializer (Vector.t A n0) with
+    | 0 => ret Vector.nil
+    | S n' => a <- deserialize ;; v <- vector_deserialize ;; ret (Vector.cons a v)
+    end.
+
+  Lemma vector_serialize_deserialize_id :
+    forall n, serialize_deserialize_id_spec vector_serialize (@vector_deserialize n).
+  Proof.
+    induction n; intros.
+    - destruct a using Vector.case0. auto.
+    - destruct a using Vector.caseS'.
+      simpl.
+      serialize_deserialize_id_crush.
+      now rewrite IHn.
+  Qed.
+
+  Global Instance vector_Serializer n : Serializer (Vector.t A n) :=
+    {| serialize := vector_serialize;
+        deserialize := vector_deserialize;
+        serialize_deserialize_id := vector_serialize_deserialize_id n
+    |}.
+
 End combinators.
+
+
+(* This has to go here because it depends on having a serializer for
+   lists available. *)
+
+Fixpoint string_to_list s :=
+  match s with
+  | String.EmptyString => nil
+  | String.String c s' => c :: (string_to_list s')
+  end.
+
+Fixpoint list_to_string l :=
+  match l with
+  | nil => String.EmptyString
+  | h::l' => String.String h (list_to_string l')
+  end.
+
+Lemma string_to_list_to_string :
+  forall s, list_to_string (string_to_list s) = s.
+Proof.
+  induction s; auto; simpl.
+  now rewrite IHs.
+Qed.
+
+Definition string_serialize (s : String.string) :=
+  serialize (string_to_list s).
+
+Definition string_deserialize : deserializer String.string :=
+  list_to_string <$> deserialize.
+
+Lemma string_serialize_deserialize_id :
+  serialize_deserialize_id_spec string_serialize string_deserialize.
+Proof.
+  unfold string_deserialize, string_serialize.
+  serialize_deserialize_id_crush.
+  now rewrite string_to_list_to_string.
+Qed.
+
+Instance string_Serializer : Serializer String.string :=
+  {| serialize := string_serialize;
+     deserialize := string_deserialize;
+     serialize_deserialize_id := string_serialize_deserialize_id
+  |}.
+
+
