BasicSerializers.v
@@ -1,0 +1,235 @@
+Require Import List ZArith.
+Import ListNotations.
+
+From StructTact Require Import StructTactics Fin.
+Require Fin Ascii.
+
+Require Import Cheerios.Core.
+Require Import Cheerios.Tactics.
+Require Import Cheerios.DeserializerMonad.
+Import DeserializerNotations.
+
+Definition bool_serialize (b : bool) : list bool := [b].
+
+Definition bool_deserialize : deserializer bool :=
+  l <- get ;;
+  match l with
+  | [] => fail
+  | b :: l' => put l' ;; ret b
+  end.
+
+Lemma bool_serialize_deserialize_id :
+  serialize_deserialize_id_spec bool_serialize bool_deserialize.
+Proof.
+  destruct a; auto.
+Qed.
+
+Instance bool_Serializer : Serializer bool :=
+  {| serialize := bool_serialize;
+     deserialize := bool_deserialize;
+     serialize_deserialize_id := bool_serialize_deserialize_id
+  |}.
+
+
+(* This is about 2x less space-efficient than necessary, since it outputs two
+   bits for every "bit" in the input, but it's very easy to verify. *)
+Fixpoint positive_serialize (p : positive) : list bool :=
+  match p with
+  | xI p' => serialize true ++ serialize true ++ positive_serialize p'
+  | xO p' => serialize true ++ serialize false ++ positive_serialize p'
+  | xH => serialize false
+  end.
+
+(* This has to be implemented directly on the implementation of Deserializer.t
+   because it performs recursion on the underlying list of bits. *)
+Fixpoint positive_deserialize (l : list bool) : option (positive * list bool) :=
+  match l with
+  | [] => None
+  | continue :: l' =>
+    if continue
+    then match l' with
+         | [] => None
+         | bit :: l' => match positive_deserialize l' with None => None
+                       | Some (p, l') => Some ((if bit then xI else xO) p, l')
+                       end
+         end
+    else Some (xH, l')
+  end.
+
+Lemma positive_serialize_deserialize_id :
+  forall p bin, positive_deserialize (positive_serialize p ++ bin) = Some (p, bin).
+Proof.
+  induction p; simpl; intros; auto; rewrite IHp; auto.
+Qed.
+
+Instance positive_Serializer : Serializer positive :=
+  {| serialize := positive_serialize;
+     deserialize := positive_deserialize;
+     serialize_deserialize_id := positive_serialize_deserialize_id
+  |}.
+
+(* This is the first example of a "typical" serializer: it combines more
+   primitive serializers (in this case, just for bool and positive) together in
+   order to serialize a Z. *)
+Definition Z_serialize (z : Z) : list bool :=
+  match z with
+  | Z0 => serialize false
+  | Zpos p => serialize true ++ serialize true ++ serialize p
+  | Zneg p => serialize true ++ serialize false ++ serialize p
+  end.
+
+Definition Z_deserialize : deserializer Z :=
+  tag <- deserialize ;;
+  match tag with
+  | true => sign <- deserialize ;;
+           (match sign with true => Zpos | false => Zneg end) <$> deserialize
+  | false => ret Z0
+  end.
+
+(* This proof is typical for serializing an algebraic datatype. Unfold the
+   serializer and deserializer, then do a case analysis and call
+   serialize_deserialize_id_crush. *)
+Lemma Z_serialize_deserialize_id :
+  serialize_deserialize_id_spec Z_serialize Z_deserialize.
+Proof.
+  unfold Z_serialize, Z_deserialize.
+  destruct a; serialize_deserialize_id_crush.
+Qed.
+
+Instance Z_Serializer : Serializer Z :=
+  {| serialize := Z_serialize;
+     deserialize := Z_deserialize;
+     serialize_deserialize_id := Z_serialize_deserialize_id
+  |}.
+
+
+Definition N_serialize (n : N) : list bool :=
+  match n with
+  | N0 => serialize false
+  | Npos p => serialize true ++ serialize p
+  end.
+
+Definition N_deserialize : deserializer N :=
+  tag <- deserialize ;;
+  match tag with
+  | false => ret N0
+  | true => Npos <$> deserialize
+  end.
+
+Lemma N_serialize_deserialize_id :
+  serialize_deserialize_id_spec N_serialize N_deserialize.
+Proof.
+  unfold N_serialize, N_deserialize.
+  destruct a; serialize_deserialize_id_crush.
+Qed.
+
+Instance N_Serializer : Serializer N :=
+  {| serialize := N_serialize;
+     deserialize := N_deserialize;
+     serialize_deserialize_id := N_serialize_deserialize_id
+  |}.
+
+
+(* The other main way to define a serializer is to use an isomorphism to another
+   type that is already serializable. *)
+Definition nat_serialize (n : nat) : list bool := serialize (N.of_nat n).
+
+Definition nat_deserialize : deserializer nat := N.to_nat <$> deserialize.
+
+(* This proof is typical for serializers defined by converting to and from a
+   type that is already serializable. Unfold the serializer and deserializer,
+   call serialize_deserialize_id_crush, and then use the proof that the
+   conversion functions are inverses. *)
+Lemma nat_serialize_deserialize_id :
+  serialize_deserialize_id_spec nat_serialize nat_deserialize.
+Proof.
+  unfold nat_serialize, nat_deserialize.
+  serialize_deserialize_id_crush.
+  now rewrite Nnat.Nat2N.id.
+Qed.
+
+Instance nat_Serializer : Serializer nat :=
+  {| serialize := nat_serialize;
+     deserialize := nat_deserialize;
+     serialize_deserialize_id := nat_serialize_deserialize_id
+  |}.
+
+
+(* Serializer for the standard library's Fin.t based on converting to nat. *)
+Definition Fin_serialize {n} (x : Fin.t n) : list bool :=
+  serialize (proj1_sig (Fin.to_nat x)).
+
+Definition Fin_deserialize {n} : deserializer (Fin.t n) :=
+  m <- deserialize ;;
+    match Fin.of_nat m n with
+    | inleft x => ret x
+    | inright _ => fail
+    end.
+
+Lemma Fin_of_nat_to_nat:
+  forall (n : nat) (a : Fin.t n), Fin.of_nat (proj1_sig (Fin.to_nat a)) n = inleft a.
+Proof.
+  induction a.
+  - auto.
+  - simpl. break_let. simpl in *.
+    now rewrite IHa.
+Qed.
+
+Lemma Fin_serialize_deserialize_id n : serialize_deserialize_id_spec Fin_serialize (@Fin_deserialize n).
+Proof.
+  unfold Fin_serialize, Fin_deserialize.
+  serialize_deserialize_id_crush.
+  now rewrite Fin_of_nat_to_nat.
+Qed.
+
+Instance Fin_Serializer n : Serializer (Fin.t n) :=
+  {| serialize := Fin_serialize;
+     deserialize := Fin_deserialize;
+     serialize_deserialize_id := Fin_serialize_deserialize_id n
+  |}.
+
+
+(* Serializer for StructTact's fin based on converting to nat. *)
+Definition fin_serialize {n} (x : fin n) : list bool :=
+  serialize (fin_to_nat x).
+
+Definition fin_deserialize {n} : deserializer (fin n) :=
+  m <- deserialize ;;
+    match fin_of_nat m n with
+    | inleft x => ret x
+    | inright _ => fail
+    end.
+
+Lemma fin_serialize_deserialize_id n : serialize_deserialize_id_spec fin_serialize (@fin_deserialize n).
+Proof.
+  unfold fin_serialize, fin_deserialize.
+  serialize_deserialize_id_crush.
+  now rewrite fin_of_nat_fin_to_nat.
+Qed.
+
+Instance fin_Serializer n : Serializer (fin n) :=
+  {| serialize := fin_serialize;
+     deserialize := fin_deserialize;
+     serialize_deserialize_id := fin_serialize_deserialize_id n
+  |}.
+
+
+Definition ascii_serialize (a : Ascii.ascii) : list bool :=
+  serialize (Ascii.nat_of_ascii a).
+
+Definition ascii_deserialize : deserializer Ascii.ascii :=
+  Ascii.ascii_of_nat <$> deserialize.
+
+Lemma ascii_serialize_deserialize_id :
+  serialize_deserialize_id_spec ascii_serialize ascii_deserialize.
+Proof.
+  unfold ascii_deserialize, ascii_serialize.
+  serialize_deserialize_id_crush.
+  now rewrite Ascii.ascii_nat_embedding.
+Qed.
+
+Instance ascii_Serializer : Serializer Ascii.ascii :=
+  {| serialize := ascii_serialize;
+     deserialize := ascii_deserialize;
+     serialize_deserialize_id := ascii_serialize_deserialize_id
+  |}.
