Examples/MorphismExample.v
@@ -1,0 +1,21 @@
+Require Import List.
+Import ListNotations.
+Require Import Vectors.Vector.
+Import VectorNotations.
+
+Require Import Cheerios.Cheerios.
+Require Import Cheerios.Morphism.
+
+(* As a simple example, we can prove that a serialized pair of two As can be
+  deserialized as a vector of As of length 2. *)
+Section silly_example.
+  Variables A : Type.
+  Variable sA : Serializer A.
+
+  Definition pair_to_vector (x : A * A) : Vector.t A 2 := [fst x; snd x].
+
+  Lemma A_to_vector_triangle : triangle_spec pair_to_vector.
+  Proof.
+    destruct a; simpl; triangle_crush.
+  Qed.
+End silly_example.
