README.md
@@ -1,2 +1,23 @@
 # Cheerios
-Formally Verified Serialization Library
+
+Cheerios is a formally verified serialization library for Coq. It
+defines a typeclass for serializable types and defines instances for
+many built-in types. The specification of a serializable type requires
+that serializing followed by deserializing is the identity.
+
+Serializers for a type A are functions `A -> list bool`.  They are
+easy to compose using list append.
+
+Deserializers for a type A are written in the monad
+`Cheerios.Deserializer.t`, which is a state monad over the binary data
+with failure. Deserializers are easy to compose using monadic sequencing.
+
+There is tactic automation (see `serialize_deserialize_id_crush`) for
+proving that user-defined serializable types are correct. Proofs of
+new serializers are typically just a few lines long.
+
+Morphisms between serializable types describe binary-level
+compatibility between the serialization format of two types. This
+allows serializing something of type A and then safely deserializing
+it at type B. There is also tactic automation for proving user-defined
+morphisms.
